proof/theories/Semantics.v
@@ -191,6 +191,7 @@ Fixpoint run_rule (rf : regfile) (is : rule_prog) (p : packet) : option verdict 
   | IExthdrReset _ _ :: rest => run_rule rf rest p (* verdict-neutral *)
   | IDup _ _ :: rest      => run_rule rf rest p   (* verdict-neutral *)
   | IObjrefMap _ _ :: rest => run_rule rf rest p  (* verdict-neutral *)
+  | ICtSetDir _ _ _ :: rest => run_rule rf rest p (* verdict-neutral *)
   | IReject t c :: _ => Some (Reject t c)
   | IQueue lo hi b f :: _ => Some (Queue lo hi b f)
   | IImmediate v :: _ => Some v
